ATL_Rule_Encoding/Apply_E2R.bpl
@@ -1,18 +1,10 @@
 /*
 rule E2R { from s : ER!Entity 
-		   to t : REL!Relation ( name  <- s.name, schema <- s.schema, attrs <- s.attrs) }
-aaa
+		   to t : REL!Relation ( name  <- s.name, attrs <- s.attrs) }
+
 */
 
-
-
-  
-
-
-procedure E2R_applys(links: Seq ref)
-requires $IsGoodHeap($tarHeap);
-requires links == NTransientLinkSet#getLinksByRule($linkHeap, _E2R);
-requires E2R_links($srcHeap,$linkHeap,$tarHeap,links);
+procedure E2R_applys();
 requires surj_tar_model($srcHeap, $tarHeap);
 requires (forall r: ref :: r!=null && read($srcHeap, r, alloc) && dtype(r) == ER$Entity ==>
 		read($tarHeap, getTarsBySrcs(Seq#Singleton(r)), alloc) 
@@ -48,11 +40,16 @@ ensures (forall<alpha> $o: ref, $f: Field alpha ::
 		((dtype($o) == REL$Relation && dtype(Seq#Index(getTarsBySrcs_inverse($o), 0)) == ER$Entity && ($f == Relation.name || $f == Relation.attrs)) || (read($tarHeap, $o, $f) == read(old($tarHeap), $o, $f))));
 ensures $HeapSucc(old($tarHeap), $tarHeap);
 ensures surj_tar_model($srcHeap, $tarHeap);
+
+implementation E2R_applys()
 {
 
 	var $i : int;
 	var link : ref;
-
+	var links: Seq ref;
+	
+	links := NTransientLinkSet#getLinksByRule($linkHeap, _E2R);
+	assume E2R_links($srcHeap,$linkHeap,$tarHeap,links);
 	
 	$i:=0;
 
