ATL_Rule_Encoding/Apply_EA2A.bpl
@@ -1,35 +1,10 @@
 /*
 rule EA2A { from att : ER!ERAttribute, ent : ER!Entity (att.entity = ent)
 	        to t : REL!RELAttribute 
-				  ( name <- att.name, isKey <- att.isKey, relation <- ent ) }
+				  ( name <- att.name, isKey <- att.isKey) }
 */
-// properties of each link of e2r rule
-function EA2A_links(
-	$srcHeap:HeapType,
-	$linkHeap:HeapType,
-	$tarHeap:HeapType,
-	links: Seq ref):bool
-{
-(forall att,ent: ref :: 
-	att!=null && read($srcHeap, att, alloc) && dtype(att) == ER$ERAttribute 
- && ent!=null && read($srcHeap, ent, alloc) && dtype(ent) == ER$Entity ==> 
-		read($srcHeap, att, ERAttribute.entity) == ent ==>
-			(exists l:ref :: l!=null &&
-				Seq#Contains(links,l) && Map#Elements(read($linkHeap, l, TransientLink#source))[_att] == att  && Map#Elements(read($linkHeap, l, TransientLink#source))[_ent] == ent ))
-&&
-(forall i: int:: 0<=i &&i <Seq#Length(links) ==>			
-			Map#Elements($linkHeap[Seq#Index(links,i), TransientLink#target])[_t] != null 
-		 && read($tarHeap, Map#Elements($linkHeap[Seq#Index(links,i), TransientLink#target])[_t], alloc)
-		 && getTarsBySrcs(Seq#Build(Seq#Singleton(Map#Elements($linkHeap[Seq#Index(links,i), TransientLink#source])[_att]), Map#Elements($linkHeap[Seq#Index(links,i), TransientLink#source])[_ent])) == Map#Elements($linkHeap[Seq#Index(links,i), TransientLink#target])[_t]
-		)
-}
 
-
-
-procedure EA2A_applys(links: Seq ref)
-requires $IsGoodHeap($tarHeap);
-requires links == NTransientLinkSet#getLinksByRule($linkHeap, _EA2A);
-requires EA2A_links($srcHeap,$linkHeap,$tarHeap,links);
+procedure EA2A_applys();
 requires surj_tar_model($srcHeap, $tarHeap);
 requires (forall att,ent: ref :: 
 	att!=null && read($srcHeap, att, alloc) && dtype(att) == ER$ERAttribute 
@@ -37,7 +12,7 @@ requires (forall att,ent: ref ::
 		read($srcHeap, att, ERAttribute.entity) == ent ==>
 		read($tarHeap, getTarsBySrcs(Seq#Build(Seq#Singleton(att),ent)), alloc) 
 	 && getTarsBySrcs(Seq#Build(Seq#Singleton(att),ent)) != null 
-	 && dtype(getTarsBySrcs(Seq#Build(Seq#Singleton(att),ent))) == REL$Relation	); // troublesome
+	 && dtype(getTarsBySrcs(Seq#Build(Seq#Singleton(att),ent))) == REL$RELAttribute	); 
 modifies $tarHeap;
 ensures (forall att,ent: ref :: 
 	att!=null && read($srcHeap, att, alloc) && dtype(att) == ER$ERAttribute 
@@ -49,26 +24,27 @@ ensures (forall att,ent: ref ::
  && ent!=null && read($srcHeap, ent, alloc) && dtype(ent) == ER$Entity ==> 
 		read($srcHeap, att, ERAttribute.entity) == ent ==>
 		read($tarHeap, getTarsBySrcs(Seq#Build(Seq#Singleton(att),ent)), RELAttribute.isKey) == read($srcHeap, att, ERAttribute.isKey));
-ensures (forall att,ent: ref :: 
-	att!=null && read($srcHeap, att, alloc) && dtype(att) == ER$ERAttribute 
- && ent!=null && read($srcHeap, ent, alloc) && dtype(ent) == ER$Entity ==> 
-		read($srcHeap, att, ERAttribute.entity) == ent ==>
-		read($tarHeap, getTarsBySrcs(Seq#Build(Seq#Singleton(att),ent)), RELAttribute.relation) == getTarsBySrcs(Seq#Singleton(ent)));
 ensures (forall<alpha> $o: ref, $f: Field alpha :: 
 	$o != null && read(old($tarHeap), $o, alloc) ==>
 		(  dtype($o) == REL$RELAttribute 
 		&& dtype(Seq#Index(getTarsBySrcs_inverse($o), 0)) == ER$ERAttribute 
 		&& dtype(Seq#Index(getTarsBySrcs_inverse($o), 1)) == ER$Entity 
-		&& ($f == RELAttribute.name || $f == RELAttribute.isKey || $f == RELAttribute.relation)) 
+		&& ($f == RELAttribute.name || $f == RELAttribute.isKey)) 
 	 || (read($tarHeap, $o, $f) == read(old($tarHeap), $o, $f)));
 ensures $HeapSucc(old($tarHeap), $tarHeap);
 ensures surj_tar_model($srcHeap, $tarHeap);
+
+implementation EA2A_applys()
 {
 
 	var $i : int;
 	var link : ref;
-
+	var links: Seq ref;
 	
+
+	links := NTransientLinkSet#getLinksByRule($linkHeap, _EA2A);
+	assume EA2A_links($srcHeap,$linkHeap,$tarHeap,links);
+
 	$i:=0;
 
 		
@@ -82,15 +58,12 @@ ensures surj_tar_model($srcHeap, $tarHeap);
 		invariant (forall i: int:: 0<=i &&i <$i ==>			
 			read($tarHeap, getTarsBySrcs(Seq#Build(Seq#Singleton(Map#Elements($linkHeap[Seq#Index(links,i), TransientLink#source])[_att]), Map#Elements($linkHeap[Seq#Index(links,i), TransientLink#source])[_ent])), RELAttribute.isKey) == $srcHeap[Map#Elements($linkHeap[Seq#Index(links,i), TransientLink#source])[_att], ERAttribute.isKey]
 		);
-		invariant (forall i: int:: 0<=i &&i <$i ==>			
-			read($tarHeap, getTarsBySrcs(Seq#Build(Seq#Singleton(Map#Elements($linkHeap[Seq#Index(links,i), TransientLink#source])[_att]), Map#Elements($linkHeap[Seq#Index(links,i), TransientLink#source])[_ent])), RELAttribute.relation) == getTarsBySrcs(Seq#Singleton(Map#Elements($linkHeap[Seq#Index(links,i), TransientLink#source])[_ent]))
-		);
 		invariant (forall<alpha> $o: ref, $f: Field alpha :: 
 	$o != null && read(old($tarHeap), $o, alloc) ==>
 		(  dtype($o) == REL$RELAttribute 
 		&& dtype(Seq#Index(getTarsBySrcs_inverse($o), 0)) == ER$ERAttribute 
 		&& dtype(Seq#Index(getTarsBySrcs_inverse($o), 1)) == ER$Entity 
-		&& ($f == RELAttribute.name || $f == RELAttribute.isKey || $f == RELAttribute.relation)) 
+		&& ($f == RELAttribute.name || $f == RELAttribute.isKey)) 
 	 || (read($tarHeap, $o, $f) == read(old($tarHeap), $o, $f)));
 		
 	{
@@ -122,13 +95,12 @@ procedure EA2A_apply (in: ref) returns ()
   modifies $tarHeap;
   ensures read($tarHeap, getTarsBySrcs(Seq#Build(Seq#Singleton(Map#Elements($linkHeap[in, TransientLink#source])[_att]), Map#Elements($linkHeap[in, TransientLink#source])[_ent])), RELAttribute.name) == read($srcHeap,Map#Elements($linkHeap[in, TransientLink#source])[_att],ERAttribute.name);
   ensures read($tarHeap, getTarsBySrcs(Seq#Build(Seq#Singleton(Map#Elements($linkHeap[in, TransientLink#source])[_att]), Map#Elements($linkHeap[in, TransientLink#source])[_ent])), RELAttribute.isKey) == read($srcHeap,Map#Elements($linkHeap[in, TransientLink#source])[_att],ERAttribute.isKey);
-  ensures read($tarHeap, getTarsBySrcs(Seq#Build(Seq#Singleton(Map#Elements($linkHeap[in, TransientLink#source])[_att]), Map#Elements($linkHeap[in, TransientLink#source])[_ent])), RELAttribute.relation) == getTarsBySrcs(Seq#Singleton(Map#Elements($linkHeap[in, TransientLink#source])[_ent]));
   ensures (forall<alpha> $o: ref, $f: Field alpha :: 
 	$o != null && read(old($tarHeap), $o, alloc) ==>
 		(  dtype($o) == REL$RELAttribute 
 		&& dtype(Seq#Index(getTarsBySrcs_inverse($o), 0)) == ER$ERAttribute 
 		&& dtype(Seq#Index(getTarsBySrcs_inverse($o), 1)) == ER$Entity 
-		&& ($f == RELAttribute.name || $f == RELAttribute.isKey || $f == RELAttribute.relation)) 
+		&& ($f == RELAttribute.name || $f == RELAttribute.isKey )) 
 	 || (read($tarHeap, $o, $f) == read(old($tarHeap), $o, $f)));
   ensures (forall<alpha> $o: ref, $f: Field alpha :: 
 	$o != null && read(old($tarHeap), $o, alloc) && $o != getTarsBySrcs(Seq#Build(Seq#Singleton(Map#Elements($linkHeap[in, TransientLink#source])[_att]), Map#Elements($linkHeap[in, TransientLink#source])[_ent])) ==> 
@@ -218,28 +190,32 @@ stk := Seq#Take(stk, Seq#Length(stk)-2);
 
 
 
-call stk := OpCode#Dup(stk);
-call stk := OpCode#GetASM(stk);
-call stk := OpCode#Load(stk, ent);
-
-call stk := ASM#Resolve(stk, $srcHeap, $Unbox(Seq#Index(stk, Seq#Length(stk)-1)): ref);
-assume $Unbox(Seq#Index(stk, Seq#Length(stk)-1)): ref == getTarsBySrcs(Seq#Singleton(Map#Elements($linkHeap[in, TransientLink#source])[_ent]));
-
-
-// set
-assert Seq#Length(stk) >= 2;
-assert $Unbox(Seq#Index(stk, Seq#Length(stk)-2)) != null;
-$tarHeap := update($tarHeap, $Unbox(Seq#Index(stk, Seq#Length(stk)-2)), 
-				FieldOfDecl(dtype($Unbox(Seq#Index(stk, Seq#Length(stk)-2))), _Field$relation): Field (ref), 
-				$Unbox(Seq#Index(stk, Seq#Length(stk)-1)));
-assume $IsGoodHeap($tarHeap);
-stk := Seq#Take(stk, Seq#Length(stk)-2);
-
-
 
 
 call stk := OpCode#Pop(stk);
 
 
 }
+
+// properties of each link of e2r rule
+function EA2A_links(
+	$srcHeap:HeapType,
+	$linkHeap:HeapType,
+	$tarHeap:HeapType,
+	links: Seq ref):bool
+{
+(forall att,ent: ref :: 
+	att!=null && read($srcHeap, att, alloc) && dtype(att) == ER$ERAttribute 
+ && ent!=null && read($srcHeap, ent, alloc) && dtype(ent) == ER$Entity ==> 
+		read($srcHeap, att, ERAttribute.entity) == ent ==>
+			(exists l:ref :: l!=null &&
+				Seq#Contains(links,l) && Map#Elements(read($linkHeap, l, TransientLink#source))[_att] == att  && Map#Elements(read($linkHeap, l, TransientLink#source))[_ent] == ent ))
+&&
+(forall i: int:: 0<=i &&i <Seq#Length(links) ==>			
+			Map#Elements($linkHeap[Seq#Index(links,i), TransientLink#target])[_t] != null 
+		 && read($tarHeap, Map#Elements($linkHeap[Seq#Index(links,i), TransientLink#target])[_t], alloc)
+		 && getTarsBySrcs(Seq#Build(Seq#Singleton(Map#Elements($linkHeap[Seq#Index(links,i), TransientLink#source])[_att]), Map#Elements($linkHeap[Seq#Index(links,i), TransientLink#source])[_ent])) == Map#Elements($linkHeap[Seq#Index(links,i), TransientLink#target])[_t]
+		)
+}
+
 
