ATL_Correctness/ER2REL_Correctness_post3.bpl
@@ -1,11 +1,3 @@
-/*
-we take two strategies to handle exists quantifier
-- rewrite exists :: f(a) -> ! (forall :: !f(a))
-- rewrite ATL rule, should not contain eopposite references
-
-*/
-
-
 function valid_src_model($h: HeapType): bool
 {
 (forall $i: ref ::
@@ -70,13 +62,13 @@ procedure driver()
 				 !read($srcHeap, $Unbox(read($srcHeap, read($srcHeap, r, Entity.attrs), IndexField(i))), ERAttribute.isKey) 
 			));
   modifies $tarHeap,$linkHeap;
-  // relations have a key
-  ensures   (forall r: ref :: r!=null && read($tarHeap, r, alloc) && dtype(r) == REL$Relation ==> 
-				dtype(Seq#Index(getTarsBySrcs_inverse(r),0)) == ER$Entity ==> // trouble some
-			!( forall i: int :: 0<=i && i<_System.array.Length(read($tarHeap, r, Relation.attrs))  ==>
-				 !read($tarHeap, $Unbox(read($tarHeap, read($tarHeap, r, Relation.attrs), IndexField(i))), RELAttribute.isKey) 
-			)
-  );
+	// attribute names unique in relation, should not hold!
+  ensures (forall $o: ref :: {read($tarHeap, $o, alloc)} $o!=null && read($tarHeap, $o, alloc) && dtype($o) == REL$Relation ==> 
+			( forall j1,j2: int :: {$Unbox(read($tarHeap, read($tarHeap, $o, Relation.attrs), IndexField(j1))): ref, $Unbox(read($tarHeap, read($tarHeap, $o, Relation.attrs), IndexField(j2))): ref} 
+			   0<=j1 && j1<j2 && j2<_System.array.Length(read($tarHeap, $o, Relation.attrs))  ==>
+				$Unbox(read($tarHeap, read($tarHeap, $o, Relation.attrs), IndexField(j1))): ref != $Unbox(read($tarHeap, read($tarHeap, $o, Relation.attrs), IndexField(j2))): ref ==>
+					read($tarHeap, $Unbox(read($tarHeap, read($tarHeap, $o, Relation.attrs), IndexField(j1))), RELAttribute.name) != read($tarHeap, $Unbox(read($tarHeap, read($tarHeap, $o, Relation.attrs), IndexField(j2))), RELAttribute.name)	
+			));
 {
 	
 	var hp: HeapType  where $IsGoodHeap(hp);
@@ -98,25 +90,10 @@ procedure driver()
 
 	call S2S_applys();
 	call E2R_applys();
-
 	call R2R_applys();
 	call EA2A_applys();
 	call RA2A_applys();
 	call RA2AK_applys();
-
-
-		
-
-// helper: rewrite the outcome of EA2A
-assume (forall r: ref :: r!=null && read($srcHeap, r, alloc) && dtype(r) == ER$Entity ==> 
-			( forall j: int :: 0<=j && j<_System.array.Length(read($srcHeap, r, Entity.attrs))  ==>
-				read($tarHeap, $Unbox(read($tarHeap, read($tarHeap, getTarsBySrcs(Seq#Singleton(r)), Relation.attrs), IndexField(j))):ref, RELAttribute.isKey) 
-				<==> 
-				read($srcHeap, $Unbox(read($srcHeap, read($srcHeap, r, Entity.attrs), IndexField(j))), ERAttribute.isKey)
-			));	 
-			
-
-
 
 
 	
@@ -129,11 +106,14 @@ ensures  (forall $o: ref :: $o == null || !read($tarHeap, $o, alloc));
 
 
 procedure S2S_match();
-requires (forall $i: ref :: $i!=null && read($srcHeap, $i, alloc) && dtype($i) == ER$ERSchema ==> 
-		getTarsBySrcs(Seq#Singleton($i))==null || !read($tarHeap, getTarsBySrcs(Seq#Singleton($i)), alloc));
+requires (forall s: ref :: s!=null && read($srcHeap, s, alloc) && dtype(s) == ER$ERSchema ==> 
+		getTarsBySrcs(Seq#Singleton(s))==null || !read($tarHeap, getTarsBySrcs(Seq#Singleton(s)), alloc));
 modifies $tarHeap,$linkHeap;
-ensures (forall $i: ref :: $i!=null && read($srcHeap, $i, alloc) && dtype($i) == ER$ERSchema ==> 
-		getTarsBySrcs(Seq#Singleton($i))!=null && read($tarHeap, getTarsBySrcs(Seq#Singleton($i)), alloc));
+ensures (forall s: ref :: s!=null && read($srcHeap, s, alloc) && dtype(s) == ER$ERSchema ==> 
+		getTarsBySrcs(Seq#Singleton(s))!=null 
+		&& read($tarHeap, getTarsBySrcs(Seq#Singleton(s)), alloc)
+		&& dtype(getTarsBySrcs(Seq#Singleton(s))) == REL$RELSchema
+		);
 ensures (forall<alpha> $o : ref, $f: Field alpha ::
 	($o == null || read($tarHeap, $o, $f) == read(old($tarHeap), $o, $f) || (dtype($o) == REL$RELSchema && dtype(Seq#Index(getTarsBySrcs_inverse($o), 0)) == ER$ERSchema && $f==alloc)));
 free ensures $HeapSucc(old($tarHeap), $tarHeap);
@@ -141,11 +121,14 @@ free ensures $HeapSucc(old($linkHeap), $linkHeap);
 free ensures surj_tar_model($srcHeap, $tarHeap);
 
 procedure E2R_match();
-requires (forall $i: ref :: $i!=null && read($srcHeap, $i, alloc) && dtype($i) == ER$Entity ==> 
-		getTarsBySrcs(Seq#Singleton($i))==null || !read($tarHeap, getTarsBySrcs(Seq#Singleton($i)), alloc));
+requires (forall s: ref :: s!=null && read($srcHeap, s, alloc) && dtype(s) == ER$Entity ==> 
+		getTarsBySrcs(Seq#Singleton(s))==null || !read($tarHeap, getTarsBySrcs(Seq#Singleton(s)), alloc));
 modifies $tarHeap,$linkHeap;
-ensures (forall $i: ref :: $i!=null && read($srcHeap, $i, alloc) && dtype($i) == ER$Entity ==> 
-		getTarsBySrcs(Seq#Singleton($i))!=null && read($tarHeap, getTarsBySrcs(Seq#Singleton($i)), alloc));
+ensures (forall s: ref :: s!=null && read($srcHeap, s, alloc) && dtype(s) == ER$Entity ==> 
+		getTarsBySrcs(Seq#Singleton(s))!=null 
+		&& read($tarHeap, getTarsBySrcs(Seq#Singleton(s)), alloc)
+		&& dtype(getTarsBySrcs(Seq#Singleton(s))) == REL$Relation
+		);
 ensures (forall<alpha> $o : ref, $f: Field alpha ::
 	($o == null || read($tarHeap, $o, $f) == read(old($tarHeap), $o, $f) || (dtype($o) == REL$Relation && dtype(Seq#Index(getTarsBySrcs_inverse($o), 0)) == ER$Entity && $f==alloc)));
 free ensures $HeapSucc(old($tarHeap), $tarHeap);
@@ -153,11 +136,14 @@ free ensures $HeapSucc(old($linkHeap), $linkHeap);
 free ensures surj_tar_model($srcHeap, $tarHeap);
 
 procedure R2R_match();
-requires (forall $i: ref :: $i!=null && read($srcHeap, $i, alloc) && dtype($i) == ER$Relship ==> 
-		getTarsBySrcs(Seq#Singleton($i))==null || !read($tarHeap, getTarsBySrcs(Seq#Singleton($i)), alloc));
+requires (forall s: ref :: s!=null && read($srcHeap, s, alloc) && dtype(s) == ER$Relship ==> 
+		getTarsBySrcs(Seq#Singleton(s))==null || !read($tarHeap, getTarsBySrcs(Seq#Singleton(s)), alloc));
 modifies $tarHeap,$linkHeap;
-ensures (forall $i: ref :: $i!=null && read($srcHeap, $i, alloc) && dtype($i) == ER$Relship ==> 
-		getTarsBySrcs(Seq#Singleton($i))!=null && read($tarHeap, getTarsBySrcs(Seq#Singleton($i)), alloc));
+ensures (forall s: ref :: s!=null && read($srcHeap, s, alloc) && dtype(s) == ER$Relship ==> 
+		getTarsBySrcs(Seq#Singleton(s))!=null 
+		&& read($tarHeap, getTarsBySrcs(Seq#Singleton(s)), alloc)
+		&& dtype(getTarsBySrcs(Seq#Singleton(s))) == REL$Relation
+		);
 ensures (forall<alpha> $o : ref, $f: Field alpha ::
 	($o == null || read($tarHeap, $o, $f) == read(old($tarHeap), $o, $f) || (dtype($o) == REL$Relation && dtype(Seq#Index(getTarsBySrcs_inverse($o), 0)) == ER$Relship && $f==alloc)));
 free ensures $HeapSucc(old($tarHeap), $tarHeap);
@@ -173,7 +159,10 @@ modifies $tarHeap,$linkHeap;
 ensures (forall att: ref :: att!=null && read($srcHeap, att, alloc) && dtype(att) == ER$ERAttribute ==> 
 			 (forall ent: ref :: ent!=null && read($srcHeap, ent, alloc) && dtype(ent) == ER$Entity ==> 
 				$srcHeap[att, ERAttribute.entity] == ent ==>
-				getTarsBySrcs(Seq#Build(Seq#Singleton(att),ent))!=null && read($tarHeap, getTarsBySrcs(Seq#Build(Seq#Singleton(att),ent)), alloc)));
+				getTarsBySrcs(Seq#Build(Seq#Singleton(att),ent))!=null 
+				&& read($tarHeap, getTarsBySrcs(Seq#Build(Seq#Singleton(att),ent)), alloc)
+				&& dtype(getTarsBySrcs(Seq#Build(Seq#Singleton(att),ent))) == REL$RELAttribute
+				));
 ensures (forall<alpha> $o : ref, $f: Field alpha ::
 	($o == null || read($tarHeap, $o, $f) == read(old($tarHeap), $o, $f) || (dtype($o) == REL$RELAttribute && dtype(Seq#Index(getTarsBySrcs_inverse($o), 0)) == ER$ERAttribute && dtype(Seq#Index(getTarsBySrcs_inverse($o), 1)) == ER$Entity && $f==alloc)));
 free ensures $HeapSucc(old($tarHeap), $tarHeap);
@@ -182,14 +171,17 @@ free ensures surj_tar_model($srcHeap, $tarHeap);
 
 procedure RA2A_match();
 requires (forall att: ref :: att!=null && read($srcHeap, att, alloc) && dtype(att) == ER$ERAttribute ==> 
-			(forall ent: ref :: ent!=null && read($srcHeap, ent, alloc) && dtype(ent) == ER$Relship ==> 
-				$srcHeap[att, ERAttribute.relship] == ent ==>
-				getTarsBySrcs(Seq#Build(Seq#Singleton(att),ent))==null || !read($tarHeap, getTarsBySrcs(Seq#Build(Seq#Singleton(att),ent)), alloc)));
+			(forall rs: ref :: rs!=null && read($srcHeap, rs, alloc) && dtype(rs) == ER$Relship ==> 
+				$srcHeap[att, ERAttribute.relship] == rs ==>
+				getTarsBySrcs(Seq#Build(Seq#Singleton(att),rs))==null || !read($tarHeap, getTarsBySrcs(Seq#Build(Seq#Singleton(att),rs)), alloc)));
 modifies $tarHeap,$linkHeap;
 ensures (forall att: ref :: att!=null && read($srcHeap, att, alloc) && dtype(att) == ER$ERAttribute ==> 
-			 (forall ent: ref :: ent!=null && read($srcHeap, ent, alloc) && dtype(ent) == ER$Relship ==> 
-				$srcHeap[att, ERAttribute.relship] == ent ==>
-				getTarsBySrcs(Seq#Build(Seq#Singleton(att),ent))!=null && read($tarHeap, getTarsBySrcs(Seq#Build(Seq#Singleton(att),ent)), alloc)));
+			 (forall rs: ref :: rs!=null && read($srcHeap, rs, alloc) && dtype(rs) == ER$Relship ==> 
+				$srcHeap[att, ERAttribute.relship] == rs ==>
+				getTarsBySrcs(Seq#Build(Seq#Singleton(att),rs))!=null 
+				&& read($tarHeap, getTarsBySrcs(Seq#Build(Seq#Singleton(att),rs)), alloc)
+				&& dtype(getTarsBySrcs(Seq#Build(Seq#Singleton(att),rs))) == REL$RELAttribute
+				));
 ensures (forall<alpha> $o : ref, $f: Field alpha ::
 	($o == null || read($tarHeap, $o, $f) == read(old($tarHeap), $o, $f) || (dtype($o) == REL$RELAttribute && dtype(Seq#Index(getTarsBySrcs_inverse($o), 0)) == ER$ERAttribute && dtype(Seq#Index(getTarsBySrcs_inverse($o), 1)) == ER$Relship && $f==alloc)));
 free ensures $HeapSucc(old($tarHeap), $tarHeap);
@@ -205,7 +197,10 @@ modifies $tarHeap,$linkHeap;
 ensures (forall att: ref :: att!=null && read($srcHeap, att, alloc) && dtype(att) == ER$ERAttribute ==> 
 			 (forall rse: ref :: rse!=null && read($srcHeap, rse, alloc) && dtype(rse) == ER$RelshipEnd ==> 
 				($srcHeap[att, ERAttribute.entity] == $srcHeap[rse, RelshipEnd.entity] && $srcHeap[att, ERAttribute.isKey]) ==>
-					getTarsBySrcs(Seq#Build(Seq#Singleton(att),rse))!=null && read($tarHeap, getTarsBySrcs(Seq#Build(Seq#Singleton(att),rse)), alloc)));
+					getTarsBySrcs(Seq#Build(Seq#Singleton(att),rse))!=null 
+					&& read($tarHeap, getTarsBySrcs(Seq#Build(Seq#Singleton(att),rse)), alloc)
+					&& dtype(getTarsBySrcs(Seq#Build(Seq#Singleton(att),rse))) == REL$RELAttribute
+					));
 ensures (forall<alpha> $o : ref, $f: Field alpha ::
 	($o == null || read($tarHeap, $o, $f) == read(old($tarHeap), $o, $f) || (dtype($o) == REL$RELAttribute && dtype(Seq#Index(getTarsBySrcs_inverse($o), 0)) == ER$ERAttribute && dtype(Seq#Index(getTarsBySrcs_inverse($o), 1)) == ER$RelshipEnd && $f==alloc)));
 free ensures $HeapSucc(old($tarHeap), $tarHeap);
@@ -213,6 +208,7 @@ free ensures $HeapSucc(old($linkHeap), $linkHeap);
 free ensures surj_tar_model($srcHeap, $tarHeap);
 
 procedure S2S_applys();
+requires surj_tar_model($srcHeap, $tarHeap);
 requires (forall r: ref :: r!=null && read($srcHeap, r, alloc) && dtype(r) == ER$ERSchema ==>
 		read($tarHeap, getTarsBySrcs(Seq#Singleton(r)), alloc) 
 	 && getTarsBySrcs(Seq#Singleton(r)) != null 
@@ -224,7 +220,7 @@ ensures (forall r: ref :: r!=null && read($srcHeap, r, alloc) && dtype(r) == ER$
 // dtype(t.relations) = class._System.array
 ensures (forall r: ref :: r!=null && read($srcHeap, r, alloc) && dtype(r) == ER$ERSchema ==> 
 	dtype(read($tarHeap, getTarsBySrcs(Seq#Singleton(r)), RELSchema.relations)) == class._System.array
-);	
+);
 // t.relations != null && t.relations.alloc
 ensures (forall r: ref :: r!=null && read($srcHeap, r, alloc) && dtype(r) == ER$ERSchema ==> 
 	read($tarHeap, getTarsBySrcs(Seq#Singleton(r)), RELSchema.relations) != null 
@@ -235,13 +231,6 @@ ensures (forall r: ref :: r!=null && read($srcHeap, r, alloc) && dtype(r) == ER$
 		_System.array.Length(read($tarHeap, getTarsBySrcs(Seq#Singleton(r)), RELSchema.relations)) 
 	 == _System.array.Length(read($srcHeap, r, ERSchema.entities))+_System.array.Length(read($srcHeap, r, ERSchema.relships))
 );
-// t.relations[j] != null t.relations[j].alloc && dtype(t.relations[j]) == REL$Relation
-ensures (forall r: ref :: r!=null && read($srcHeap, r, alloc) && dtype(r) == ER$ERSchema ==> 
-			( forall j: int :: 0<=j && j<_System.array.Length(read($tarHeap, getTarsBySrcs(Seq#Singleton(r)), RELSchema.relations))  ==>
-				$Unbox(read($tarHeap, read($tarHeap, getTarsBySrcs(Seq#Singleton(r)), RELSchema.relations), IndexField(j))): ref != null
-			 &&	read($tarHeap, $Unbox(read($tarHeap, read($tarHeap, getTarsBySrcs(Seq#Singleton(r)), RELSchema.relations), IndexField(j))): ref, alloc)
-			 && dtype($Unbox(read($tarHeap, read($tarHeap, getTarsBySrcs(Seq#Singleton(r)), RELSchema.relations), IndexField(j))): ref) == REL$Relation
-			));
 // t.relations[j] == s.entities[j]
 ensures (forall r: ref :: r!=null && read($srcHeap, r, alloc) && dtype(r) == ER$ERSchema ==> 
 			( forall j: int :: 0<=j && j<_System.array.Length(read($srcHeap, r, ERSchema.entities))  ==>
@@ -254,28 +243,17 @@ ensures (forall r: ref :: r!=null && read($srcHeap, r, alloc) && dtype(r) == ER$
 				$Unbox(read($tarHeap, read($tarHeap, getTarsBySrcs(Seq#Singleton(r)), RELSchema.relations), IndexField(j+_System.array.Length(read($srcHeap, r, ERSchema.entities))))): ref ==
 				getTarsBySrcs(Seq#Singleton( $Unbox(read($srcHeap, read($srcHeap, r, ERSchema.relships), IndexField(j))): ref) )
 			));
-// frame property, i.e. what is changed / not changed.
-// [todo: feel under-specified here] the array element is also changed, effected on field [IndexField], i.e.:
-// (exists k: int :: 0 <= k && k < _System.array.Length([t.relations]) && $o == [t.relations] && $f == IndexField(k))
+// frame
 ensures (forall<alpha> $o: ref, $f: Field alpha :: 
 	$o != null && read(old($tarHeap), $o, alloc) ==>
 		( (dtype($o) == REL$RELSchema && dtype(Seq#Index(getTarsBySrcs_inverse($o), 0)) == ER$ERSchema && ($f == RELSchema.name || $f == RELSchema.relations)) || (read($tarHeap, $o, $f) == read(old($tarHeap), $o, $f))));
 ensures $HeapSucc(old($tarHeap), $tarHeap);
-free ensures surj_tar_model($srcHeap, $tarHeap);
+ensures surj_tar_model($srcHeap, $tarHeap);
 		
-/* redundant
-ensures   (forall r: ref :: r!=null && read($srcHeap, r, alloc) && dtype(r) == ER$ERSchema ==>
-				getTarsBySrcs(Seq#Singleton(r)) != null && dtype(getTarsBySrcs(Seq#Singleton(r))) == REL$RELSchema	);
-// this is conveyed by E2R rule.
-ensures (forall r: ref :: r!=null && read($srcHeap, r, alloc) && dtype(r) == ER$ERSchema ==> 
-			( forall j: int :: 0<=j && j<_System.array.Length(read($tarHeap, getTarsBySrcs(Seq#Singleton(r)), RELSchema.relations))  ==>
-				dtype($Unbox(read($tarHeap, read($tarHeap, getTarsBySrcs(Seq#Singleton(r)), RELSchema.relations), IndexField(j))): ref) ==
-				REL$Relation
-			));							
-*/
 
 
 procedure E2R_applys();
+requires surj_tar_model($srcHeap, $tarHeap);
 requires (forall r: ref :: r!=null && read($srcHeap, r, alloc) && dtype(r) == ER$Entity ==>
 		read($tarHeap, getTarsBySrcs(Seq#Singleton(r)), alloc) 
 	 && getTarsBySrcs(Seq#Singleton(r)) != null 
@@ -312,6 +290,7 @@ ensures $HeapSucc(old($tarHeap), $tarHeap);
 ensures surj_tar_model($srcHeap, $tarHeap);
 
 procedure R2R_applys();
+requires surj_tar_model($srcHeap, $tarHeap);
 requires (forall r: ref :: r!=null && read($srcHeap, r, alloc) && dtype(r) == ER$Relship ==>
 		read($tarHeap, getTarsBySrcs(Seq#Singleton(r)), alloc) 
 	 && getTarsBySrcs(Seq#Singleton(r)) != null 
@@ -325,16 +304,18 @@ ensures (forall<alpha> $o: ref, $f: Field alpha ::
 	$o != null && read(old($tarHeap), $o, alloc) ==>
 		((dtype($o) == REL$Relation && dtype(Seq#Index(getTarsBySrcs_inverse($o), 0)) == ER$Relship && $f == Relation.name) || (read($tarHeap, $o, $f) == read(old($tarHeap), $o, $f))));
 ensures $HeapSucc(old($tarHeap), $tarHeap);
-free ensures surj_tar_model($srcHeap, $tarHeap);
+ensures surj_tar_model($srcHeap, $tarHeap);
 
 
 procedure EA2A_applys();
+requires surj_tar_model($srcHeap, $tarHeap);
 requires (forall att,ent: ref :: 
 	att!=null && read($srcHeap, att, alloc) && dtype(att) == ER$ERAttribute 
  && ent!=null && read($srcHeap, ent, alloc) && dtype(ent) == ER$Entity ==> 
 		read($srcHeap, att, ERAttribute.entity) == ent ==>
 		read($tarHeap, getTarsBySrcs(Seq#Build(Seq#Singleton(att),ent)), alloc) 
-	 && getTarsBySrcs(Seq#Build(Seq#Singleton(att),ent)) != null ); 
+	 && getTarsBySrcs(Seq#Build(Seq#Singleton(att),ent)) != null 
+	 && dtype(getTarsBySrcs(Seq#Build(Seq#Singleton(att),ent))) == REL$RELAttribute	); 
 modifies $tarHeap;
 ensures (forall att,ent: ref :: 
 	att!=null && read($srcHeap, att, alloc) && dtype(att) == ER$ERAttribute 
@@ -357,12 +338,14 @@ ensures $HeapSucc(old($tarHeap), $tarHeap);
 ensures surj_tar_model($srcHeap, $tarHeap);
 
 procedure RA2A_applys();
+requires surj_tar_model($srcHeap, $tarHeap);
 requires (forall att,rs: ref :: 
 	att!=null && read($srcHeap, att, alloc) && dtype(att) == ER$ERAttribute 
  && rs!=null && read($srcHeap, rs, alloc) && dtype(rs) == ER$Relship ==> 
 		read($srcHeap, att, ERAttribute.relship) == rs ==>
 		read($tarHeap, getTarsBySrcs(Seq#Build(Seq#Singleton(att),rs)), alloc) 
-	 && getTarsBySrcs(Seq#Build(Seq#Singleton(att),rs)) != null );
+	 && getTarsBySrcs(Seq#Build(Seq#Singleton(att),rs)) != null 
+	 && dtype(getTarsBySrcs(Seq#Build(Seq#Singleton(att),rs))) == REL$RELAttribute	);	
 modifies $tarHeap;
 ensures (forall att,rs: ref :: 
 	att!=null && read($srcHeap, att, alloc) && dtype(att) == ER$ERAttribute 
@@ -390,33 +373,35 @@ ensures $HeapSucc(old($tarHeap), $tarHeap);
 ensures surj_tar_model($srcHeap, $tarHeap);
 
 procedure RA2AK_applys();
-requires (forall att,rse: ref :: 
+requires surj_tar_model($srcHeap, $tarHeap);
+requires (forall att,rs: ref :: 
 	att!=null && read($srcHeap, att, alloc) && dtype(att) == ER$ERAttribute 
- && rse!=null && read($srcHeap, rse, alloc) && dtype(rse) == ER$RelshipEnd ==> 
-		read($srcHeap, att, ERAttribute.entity) == read($srcHeap,rse, RelshipEnd.entity) && read($srcHeap,att,ERAttribute.isKey) ==>
-		read($tarHeap, getTarsBySrcs(Seq#Build(Seq#Singleton(att),rse)), alloc) 
-	 && getTarsBySrcs(Seq#Build(Seq#Singleton(att),rse)) != null ); 
+ && rs!=null && read($srcHeap, rs, alloc) && dtype(rs) == ER$Relship ==> 
+		read($srcHeap, att, ERAttribute.relship) == rs ==>
+		read($tarHeap, getTarsBySrcs(Seq#Build(Seq#Singleton(att),rs)), alloc) 
+	 && getTarsBySrcs(Seq#Build(Seq#Singleton(att),rs)) != null 
+	 && dtype(getTarsBySrcs(Seq#Build(Seq#Singleton(att),rs))) == REL$RELAttribute	);	
 modifies $tarHeap;
-ensures (forall att,rse: ref :: 
+ensures (forall att,rs: ref :: 
 	att!=null && read($srcHeap, att, alloc) && dtype(att) == ER$ERAttribute 
- && rse!=null && read($srcHeap, rse, alloc) && dtype(rse) == ER$RelshipEnd ==> 
-		read($srcHeap, att, ERAttribute.entity) == read($srcHeap,rse, RelshipEnd.entity) && read($srcHeap,att,ERAttribute.isKey) ==>
-		read($tarHeap, getTarsBySrcs(Seq#Build(Seq#Singleton(att),rse)), RELAttribute.name) == read($srcHeap, att, ERAttribute.name));
-ensures (forall att,rse: ref :: 
+ && rs!=null && read($srcHeap, rs, alloc) && dtype(rs) == ER$Relship ==> 
+		read($srcHeap, att, ERAttribute.relship) == rs ==>
+		read($tarHeap, getTarsBySrcs(Seq#Build(Seq#Singleton(att),rs)), RELAttribute.name) == read($srcHeap, att, ERAttribute.name));
+ensures (forall att,rs: ref :: 
 	att!=null && read($srcHeap, att, alloc) && dtype(att) == ER$ERAttribute 
- && rse!=null && read($srcHeap, rse, alloc) && dtype(rse) == ER$RelshipEnd ==> 
-		read($srcHeap, att, ERAttribute.entity) == read($srcHeap,rse, RelshipEnd.entity) && read($srcHeap,att,ERAttribute.isKey) ==>
-		read($tarHeap, getTarsBySrcs(Seq#Build(Seq#Singleton(att),rse)), RELAttribute.isKey) == read($srcHeap, att, ERAttribute.isKey));
-ensures (forall att,rse: ref :: 
+ && rs!=null && read($srcHeap, rs, alloc) && dtype(rs) == ER$Relship ==> 
+		read($srcHeap, att, ERAttribute.relship) == rs ==>
+		read($tarHeap, getTarsBySrcs(Seq#Build(Seq#Singleton(att),rs)), RELAttribute.isKey) == read($srcHeap, att, ERAttribute.isKey));
+ensures (forall att,rs: ref :: 
 	att!=null && read($srcHeap, att, alloc) && dtype(att) == ER$ERAttribute 
- && rse!=null && read($srcHeap, rse, alloc) && dtype(rse) == ER$RelshipEnd ==> 
-		read($srcHeap, att, ERAttribute.entity) == read($srcHeap,rse, RelshipEnd.entity) && read($srcHeap,att,ERAttribute.isKey) ==>
-		read($tarHeap, getTarsBySrcs(Seq#Build(Seq#Singleton(att),rse)), RELAttribute.relation) == getTarsBySrcs(Seq#Singleton(read($srcHeap,rse,RelshipEnd.relship))));
+ && rs!=null && read($srcHeap, rs, alloc) && dtype(rs) == ER$Relship ==> 
+		read($srcHeap, att, ERAttribute.relship) == rs ==>
+		read($tarHeap, getTarsBySrcs(Seq#Build(Seq#Singleton(att),rs)), RELAttribute.relation) == getTarsBySrcs(Seq#Singleton(rs)));
 ensures (forall<alpha> $o: ref, $f: Field alpha :: 
 	$o != null && read(old($tarHeap), $o, alloc) ==>
 		(  dtype($o) == REL$RELAttribute 
 		&& dtype(Seq#Index(getTarsBySrcs_inverse($o), 0)) == ER$ERAttribute 
-		&& dtype(Seq#Index(getTarsBySrcs_inverse($o), 1)) == ER$RelshipEnd 
+		&& dtype(Seq#Index(getTarsBySrcs_inverse($o), 1)) == ER$Relship 
 		&& ($f == RELAttribute.name || $f == RELAttribute.isKey || $f == RELAttribute.relation)) 
 	 || (read($tarHeap, $o, $f) == read(old($tarHeap), $o, $f)));
 ensures $HeapSucc(old($tarHeap), $tarHeap);
