ATL_Correctness/ER2REL_Correctness_post4.bpl
@@ -1,0 +1,426 @@
+
+
+
+function valid_src_model($h: HeapType): bool
+{
+(forall $i: ref ::
+	
+	($i!=null && read($h, $i, alloc) && dtype($i) == ER$ERSchema ==> 
+	 // ER$ERSchema => its [entities] feature is not null, and every of them is type of [ER$Entity], not [null], and is [allocated]
+		( read($h, $i, ERSchema.entities)!=null &&
+		 (forall j: int :: 0<=j && j<_System.array.Length(read($h, $i, ERSchema.entities)) ==> 
+		    ($Unbox(read($h, read($h, $i, ERSchema.entities), IndexField(j))): ref !=null 
+		      && read($h, $Unbox(read($h, read($h, $i, ERSchema.entities), IndexField(j))): ref, alloc)
+		      && dtype($Unbox(read($h, read($h, $i, ERSchema.entities), IndexField(j))): ref)==ER$Entity) ))
+	 // ER$ERSchema => its [relships] feature is not null, and every of them is type of [ER$Relship], not [null], and is [allocated]
+	 && ( read($h, $i, ERSchema.relships)!=null &&
+		 (forall j: int :: 0<=j && j<_System.array.Length(read($h, $i, ERSchema.relships)) ==> 
+		    ($Unbox(read($h, read($h, $i, ERSchema.relships), IndexField(j))): ref !=null 
+		      && read($h, $Unbox(read($h, read($h, $i, ERSchema.relships), IndexField(j))): ref, alloc)
+		      && dtype($Unbox(read($h, read($h, $i, ERSchema.relships), IndexField(j))): ref)==ER$Relship) ))
+	)
+)
+}
+
+procedure driver()
+  requires valid_src_model($srcHeap);
+  // unique schema names
+  requires (forall $i1, $i2: ref :: $i1!=$i2 && $i1!=null && read($srcHeap, $i1, alloc) && dtype($i1) == ER$ERSchema
+				&& $i2!=null && read($srcHeap, $i2, alloc) && dtype($i2) == ER$ERSchema ==>
+				read($srcHeap, $i1, ERSchema.name) != read($srcHeap, $i2, ERSchema.name));
+  // entity names are unique in schema
+  requires (forall r: ref :: r!=null && read($srcHeap, r, alloc) && dtype(r) == ER$ERSchema ==> 
+			( forall j1,j2: int :: 0<=j1 && j1<j2 && j2<_System.array.Length(read($srcHeap, r, ERSchema.entities))  ==>
+				$Unbox(read($srcHeap, read($srcHeap, r, ERSchema.entities), IndexField(j1))): ref != $Unbox(read($srcHeap, read($srcHeap, r, ERSchema.entities), IndexField(j2))): ref ==>
+				read($srcHeap, $Unbox(read($srcHeap, read($srcHeap, r, ERSchema.entities), IndexField(j1))), Entity.name) != read($srcHeap, $Unbox(read($srcHeap, read($srcHeap, r, ERSchema.entities), IndexField(j2))), Entity.name)
+			));
+  // relship names are unique in schema
+  requires (forall r: ref :: r!=null && read($srcHeap, r, alloc) && dtype(r) == ER$ERSchema ==> 
+			( forall j1,j2: int :: 0<=j1 && j1<j2 && j2<_System.array.Length(read($srcHeap, r, ERSchema.relships))  ==>
+				$Unbox(read($srcHeap, read($srcHeap, r, ERSchema.relships), IndexField(j1))): ref != $Unbox(read($srcHeap, read($srcHeap, r, ERSchema.relships), IndexField(j2))): ref ==>
+				read($srcHeap, $Unbox(read($srcHeap, read($srcHeap, r, ERSchema.relships), IndexField(j1))), Relship.name) != read($srcHeap, $Unbox(read($srcHeap, read($srcHeap, r, ERSchema.relships), IndexField(j2))), Relship.name)
+			));
+  // disjoint entity and relship names
+  requires (forall r: ref :: r!=null && read($srcHeap, r, alloc) && dtype(r) == ER$ERSchema ==> 
+			( forall i: int :: 0<=i && i<_System.array.Length(read($srcHeap, r, ERSchema.entities))  ==>
+			 ( forall j: int :: 0<=j && j<_System.array.Length(read($srcHeap, r, ERSchema.relships))  ==>
+				$Unbox(read($srcHeap, read($srcHeap, r, ERSchema.entities), IndexField(i))): ref != $Unbox(read($srcHeap, read($srcHeap, r, ERSchema.relships), IndexField(j))): ref ==>
+				read($srcHeap, $Unbox(read($srcHeap, read($srcHeap, r, ERSchema.entities), IndexField(i))), Entity.name) != read($srcHeap, $Unbox(read($srcHeap, read($srcHeap, r, ERSchema.relships), IndexField(j))), Relship.name)
+			)));
+  // attr names are unique in entity
+  requires (forall r: ref :: r!=null && read($srcHeap, r, alloc) && dtype(r) == ER$Entity ==> 
+			( forall j1,j2: int :: 0<=j1 && j1<j2 && j2<_System.array.Length(read($srcHeap, r, Entity.attrs))  ==>
+				$Unbox(read($srcHeap, read($srcHeap, r, Entity.attrs), IndexField(j1))): ref != $Unbox(read($srcHeap, read($srcHeap, r, Entity.attrs), IndexField(j2))): ref ==>
+				read($srcHeap, $Unbox(read($srcHeap, read($srcHeap, r, Entity.attrs), IndexField(j1))), ERAttribute.name) != read($srcHeap, $Unbox(read($srcHeap, read($srcHeap, r, Entity.attrs), IndexField(j2))), ERAttribute.name)
+			));
+  // attr names are unique in relship
+  requires (forall r: ref :: r!=null && read($srcHeap, r, alloc) && dtype(r) == ER$Relship ==> 
+			( forall j1,j2: int :: 0<=j1 && j1<j2 && j2<_System.array.Length(read($srcHeap, r, Relship.attrs))  ==>
+				$Unbox(read($srcHeap, read($srcHeap, r, Relship.attrs), IndexField(j1))): ref != $Unbox(read($srcHeap, read($srcHeap, r, Relship.attrs), IndexField(j2))): ref ==>
+				read($srcHeap, $Unbox(read($srcHeap, read($srcHeap, r, Relship.attrs), IndexField(j1))), ERAttribute.name) != read($srcHeap, $Unbox(read($srcHeap, read($srcHeap, r, Relship.attrs), IndexField(j2))), ERAttribute.name)
+			));
+  // entities have a key
+  requires (forall r: ref :: r!=null && read($srcHeap, r, alloc) && dtype(r) == ER$Entity ==> 
+			!( forall i: int :: 0<=i && i<_System.array.Length(read($srcHeap, r, Entity.attrs))  ==>
+				 !read($srcHeap, $Unbox(read($srcHeap, read($srcHeap, r, Entity.attrs), IndexField(i))), ERAttribute.isKey) 
+			));
+  modifies $tarHeap,$linkHeap;
+  // relations have a key
+  ensures   (forall r: ref :: r!=null && read($tarHeap, r, alloc) && dtype(r) == REL$Relation ==> 
+				dtype(Seq#Index(getTarsBySrcs_inverse(r),0)) == ER$Entity ==> // trouble some
+			!( forall i: int :: 0<=i && i<_System.array.Length(read($tarHeap, r, Relation.attrs))  ==>
+				 !read($tarHeap, $Unbox(read($tarHeap, read($tarHeap, r, Relation.attrs), IndexField(i))), RELAttribute.isKey) 
+			)
+  );
+{
+	
+	var hp: HeapType  where $IsGoodHeap(hp);
+
+
+	
+
+	call init_tar_model(); 
+	
+
+	call S2S_match();
+	call E2R_match();
+	call R2R_match();
+	call EA2A_match();
+	call RA2A_match();
+	call RA2AK_match();
+
+
+
+	call S2S_applys();
+	call E2R_applys();
+
+	call R2R_applys();
+	call EA2A_applys();
+	call RA2A_applys();
+	call RA2AK_applys();
+
+
+		
+
+// helper: rewrite the outcome of EA2A
+assume (forall r: ref :: r!=null && read($srcHeap, r, alloc) && dtype(r) == ER$Entity ==> 
+			( forall j: int :: 0<=j && j<_System.array.Length(read($srcHeap, r, Entity.attrs))  ==>
+				read($tarHeap, $Unbox(read($tarHeap, read($tarHeap, getTarsBySrcs(Seq#Singleton(r)), Relation.attrs), IndexField(j))):ref, RELAttribute.isKey) 
+				<==> 
+				read($srcHeap, $Unbox(read($srcHeap, read($srcHeap, r, Entity.attrs), IndexField(j))), ERAttribute.isKey)
+			));	 
+			
+
+
+
+
+	
+}
+
+// the outcome of init is that: no rule to handle src tuple in ATL spec will return null, or not allocated yet.
+procedure init_tar_model();
+modifies $tarHeap;
+ensures  (forall $o: ref :: $o == null || !read($tarHeap, $o, alloc));
+
+
+procedure S2S_match();
+requires (forall s: ref :: s!=null && read($srcHeap, s, alloc) && dtype(s) == ER$ERSchema ==> 
+		getTarsBySrcs(Seq#Singleton(s))==null || !read($tarHeap, getTarsBySrcs(Seq#Singleton(s)), alloc));
+modifies $tarHeap,$linkHeap;
+ensures (forall s: ref :: s!=null && read($srcHeap, s, alloc) && dtype(s) == ER$ERSchema ==> 
+		getTarsBySrcs(Seq#Singleton(s))!=null 
+		&& read($tarHeap, getTarsBySrcs(Seq#Singleton(s)), alloc)
+		&& dtype(getTarsBySrcs(Seq#Singleton(s))) == REL$RELSchema
+		);
+ensures (forall<alpha> $o : ref, $f: Field alpha ::
+	($o == null || read($tarHeap, $o, $f) == read(old($tarHeap), $o, $f) || (dtype($o) == REL$RELSchema && dtype(Seq#Index(getTarsBySrcs_inverse($o), 0)) == ER$ERSchema && $f==alloc)));
+free ensures $HeapSucc(old($tarHeap), $tarHeap);
+free ensures $HeapSucc(old($linkHeap), $linkHeap);
+free ensures surj_tar_model($srcHeap, $tarHeap);
+
+procedure E2R_match();
+requires (forall s: ref :: s!=null && read($srcHeap, s, alloc) && dtype(s) == ER$Entity ==> 
+		getTarsBySrcs(Seq#Singleton(s))==null || !read($tarHeap, getTarsBySrcs(Seq#Singleton(s)), alloc));
+modifies $tarHeap,$linkHeap;
+ensures (forall s: ref :: s!=null && read($srcHeap, s, alloc) && dtype(s) == ER$Entity ==> 
+		getTarsBySrcs(Seq#Singleton(s))!=null 
+		&& read($tarHeap, getTarsBySrcs(Seq#Singleton(s)), alloc)
+		&& dtype(getTarsBySrcs(Seq#Singleton(s))) == REL$Relation
+		);
+ensures (forall<alpha> $o : ref, $f: Field alpha ::
+	($o == null || read($tarHeap, $o, $f) == read(old($tarHeap), $o, $f) || (dtype($o) == REL$Relation && dtype(Seq#Index(getTarsBySrcs_inverse($o), 0)) == ER$Entity && $f==alloc)));
+free ensures $HeapSucc(old($tarHeap), $tarHeap);
+free ensures $HeapSucc(old($linkHeap), $linkHeap);
+free ensures surj_tar_model($srcHeap, $tarHeap);
+
+procedure R2R_match();
+requires (forall s: ref :: s!=null && read($srcHeap, s, alloc) && dtype(s) == ER$Relship ==> 
+		getTarsBySrcs(Seq#Singleton(s))==null || !read($tarHeap, getTarsBySrcs(Seq#Singleton(s)), alloc));
+modifies $tarHeap,$linkHeap;
+ensures (forall s: ref :: s!=null && read($srcHeap, s, alloc) && dtype(s) == ER$Relship ==> 
+		getTarsBySrcs(Seq#Singleton(s))!=null 
+		&& read($tarHeap, getTarsBySrcs(Seq#Singleton(s)), alloc)
+		&& dtype(getTarsBySrcs(Seq#Singleton(s))) == REL$Relation
+		);
+ensures (forall<alpha> $o : ref, $f: Field alpha ::
+	($o == null || read($tarHeap, $o, $f) == read(old($tarHeap), $o, $f) || (dtype($o) == REL$Relation && dtype(Seq#Index(getTarsBySrcs_inverse($o), 0)) == ER$Relship && $f==alloc)));
+free ensures $HeapSucc(old($tarHeap), $tarHeap);
+free ensures $HeapSucc(old($linkHeap), $linkHeap);
+free ensures surj_tar_model($srcHeap, $tarHeap);
+
+procedure EA2A_match();
+requires (forall att: ref :: att!=null && read($srcHeap, att, alloc) && dtype(att) == ER$ERAttribute ==> 
+			(forall ent: ref :: ent!=null && read($srcHeap, ent, alloc) && dtype(ent) == ER$Entity ==> 
+				$srcHeap[att, ERAttribute.entity] == ent ==>
+				getTarsBySrcs(Seq#Build(Seq#Singleton(att),ent))==null || !read($tarHeap, getTarsBySrcs(Seq#Build(Seq#Singleton(att),ent)), alloc)));
+modifies $tarHeap,$linkHeap;
+ensures (forall att: ref :: att!=null && read($srcHeap, att, alloc) && dtype(att) == ER$ERAttribute ==> 
+			 (forall ent: ref :: ent!=null && read($srcHeap, ent, alloc) && dtype(ent) == ER$Entity ==> 
+				$srcHeap[att, ERAttribute.entity] == ent ==>
+				getTarsBySrcs(Seq#Build(Seq#Singleton(att),ent))!=null 
+				&& read($tarHeap, getTarsBySrcs(Seq#Build(Seq#Singleton(att),ent)), alloc)
+				&& dtype(getTarsBySrcs(Seq#Build(Seq#Singleton(att),ent))) == REL$RELAttribute
+				));
+ensures (forall<alpha> $o : ref, $f: Field alpha ::
+	($o == null || read($tarHeap, $o, $f) == read(old($tarHeap), $o, $f) || (dtype($o) == REL$RELAttribute && dtype(Seq#Index(getTarsBySrcs_inverse($o), 0)) == ER$ERAttribute && dtype(Seq#Index(getTarsBySrcs_inverse($o), 1)) == ER$Entity && $f==alloc)));
+free ensures $HeapSucc(old($tarHeap), $tarHeap);
+free ensures $HeapSucc(old($linkHeap), $linkHeap);
+free ensures surj_tar_model($srcHeap, $tarHeap);
+
+procedure RA2A_match();
+requires (forall att: ref :: att!=null && read($srcHeap, att, alloc) && dtype(att) == ER$ERAttribute ==> 
+			(forall rs: ref :: rs!=null && read($srcHeap, rs, alloc) && dtype(rs) == ER$Relship ==> 
+				$srcHeap[att, ERAttribute.relship] == rs ==>
+				getTarsBySrcs(Seq#Build(Seq#Singleton(att),rs))==null || !read($tarHeap, getTarsBySrcs(Seq#Build(Seq#Singleton(att),rs)), alloc)));
+modifies $tarHeap,$linkHeap;
+ensures (forall att: ref :: att!=null && read($srcHeap, att, alloc) && dtype(att) == ER$ERAttribute ==> 
+			 (forall rs: ref :: rs!=null && read($srcHeap, rs, alloc) && dtype(rs) == ER$Relship ==> 
+				$srcHeap[att, ERAttribute.relship] == rs ==>
+				getTarsBySrcs(Seq#Build(Seq#Singleton(att),rs))!=null 
+				&& read($tarHeap, getTarsBySrcs(Seq#Build(Seq#Singleton(att),rs)), alloc)
+				&& dtype(getTarsBySrcs(Seq#Build(Seq#Singleton(att),rs))) == REL$RELAttribute
+				));
+ensures (forall<alpha> $o : ref, $f: Field alpha ::
+	($o == null || read($tarHeap, $o, $f) == read(old($tarHeap), $o, $f) || (dtype($o) == REL$RELAttribute && dtype(Seq#Index(getTarsBySrcs_inverse($o), 0)) == ER$ERAttribute && dtype(Seq#Index(getTarsBySrcs_inverse($o), 1)) == ER$Relship && $f==alloc)));
+free ensures $HeapSucc(old($tarHeap), $tarHeap);
+free ensures $HeapSucc(old($linkHeap), $linkHeap);
+free ensures surj_tar_model($srcHeap, $tarHeap);
+
+procedure RA2AK_match();
+requires (forall att: ref :: att!=null && read($srcHeap, att, alloc) && dtype(att) == ER$ERAttribute ==> 
+			(forall rse: ref :: rse!=null && read($srcHeap, rse, alloc) && dtype(rse) == ER$RelshipEnd ==> 
+				($srcHeap[att, ERAttribute.entity] == $srcHeap[rse, RelshipEnd.entity] && $srcHeap[att, ERAttribute.isKey]) ==>
+					getTarsBySrcs(Seq#Build(Seq#Singleton(att),rse))==null || !read($tarHeap, getTarsBySrcs(Seq#Build(Seq#Singleton(att),rse)), alloc)));
+modifies $tarHeap,$linkHeap;
+ensures (forall att: ref :: att!=null && read($srcHeap, att, alloc) && dtype(att) == ER$ERAttribute ==> 
+			 (forall rse: ref :: rse!=null && read($srcHeap, rse, alloc) && dtype(rse) == ER$RelshipEnd ==> 
+				($srcHeap[att, ERAttribute.entity] == $srcHeap[rse, RelshipEnd.entity] && $srcHeap[att, ERAttribute.isKey]) ==>
+					getTarsBySrcs(Seq#Build(Seq#Singleton(att),rse))!=null 
+					&& read($tarHeap, getTarsBySrcs(Seq#Build(Seq#Singleton(att),rse)), alloc)
+					&& dtype(getTarsBySrcs(Seq#Build(Seq#Singleton(att),rse))) == REL$RELAttribute
+					));
+ensures (forall<alpha> $o : ref, $f: Field alpha ::
+	($o == null || read($tarHeap, $o, $f) == read(old($tarHeap), $o, $f) || (dtype($o) == REL$RELAttribute && dtype(Seq#Index(getTarsBySrcs_inverse($o), 0)) == ER$ERAttribute && dtype(Seq#Index(getTarsBySrcs_inverse($o), 1)) == ER$RelshipEnd && $f==alloc)));
+free ensures $HeapSucc(old($tarHeap), $tarHeap);
+free ensures $HeapSucc(old($linkHeap), $linkHeap);
+free ensures surj_tar_model($srcHeap, $tarHeap);
+
+procedure S2S_applys();
+requires surj_tar_model($srcHeap, $tarHeap);
+requires (forall r: ref :: r!=null && read($srcHeap, r, alloc) && dtype(r) == ER$ERSchema ==>
+		read($tarHeap, getTarsBySrcs(Seq#Singleton(r)), alloc) 
+	 && getTarsBySrcs(Seq#Singleton(r)) != null 
+	 && dtype(getTarsBySrcs(Seq#Singleton(r))) == REL$RELSchema	);
+modifies $tarHeap;
+// t.name <- s.name
+ensures (forall r: ref :: r!=null && read($srcHeap, r, alloc) && dtype(r) == ER$ERSchema ==> 
+		read($tarHeap, getTarsBySrcs(Seq#Singleton(r)), RELSchema.name) == read($srcHeap, r, ERSchema.name));
+// dtype(t.relations) = class._System.array
+ensures (forall r: ref :: r!=null && read($srcHeap, r, alloc) && dtype(r) == ER$ERSchema ==> 
+	dtype(read($tarHeap, getTarsBySrcs(Seq#Singleton(r)), RELSchema.relations)) == class._System.array
+);
+// t.relations != null && t.relations.alloc
+ensures (forall r: ref :: r!=null && read($srcHeap, r, alloc) && dtype(r) == ER$ERSchema ==> 
+	read($tarHeap, getTarsBySrcs(Seq#Singleton(r)), RELSchema.relations) != null 
+ && read($tarHeap, read($tarHeap, getTarsBySrcs(Seq#Singleton(r)), RELSchema.relations), alloc)
+);
+// length(t.relations) = length(s.entities)+length(s.relships)
+ensures (forall r: ref :: r!=null && read($srcHeap, r, alloc) && dtype(r) == ER$ERSchema ==> 
+		_System.array.Length(read($tarHeap, getTarsBySrcs(Seq#Singleton(r)), RELSchema.relations)) 
+	 == _System.array.Length(read($srcHeap, r, ERSchema.entities))+_System.array.Length(read($srcHeap, r, ERSchema.relships))
+);
+// t.relations[j] == s.entities[j]
+ensures (forall r: ref :: r!=null && read($srcHeap, r, alloc) && dtype(r) == ER$ERSchema ==> 
+			( forall j: int :: 0<=j && j<_System.array.Length(read($srcHeap, r, ERSchema.entities))  ==>
+				$Unbox(read($tarHeap, read($tarHeap, getTarsBySrcs(Seq#Singleton(r)), RELSchema.relations), IndexField(j))): ref ==
+				getTarsBySrcs(Seq#Singleton( $Unbox(read($srcHeap, read($srcHeap, r, ERSchema.entities), IndexField(j))): ref) )
+			));
+// t.relations[j+len(s.entities)] == s.relships[j]
+ensures (forall r: ref :: r!=null && read($srcHeap, r, alloc) && dtype(r) == ER$ERSchema ==> 
+			( forall j: int :: 0<=j && j<_System.array.Length(read($srcHeap, r, ERSchema.relships))  ==>
+				$Unbox(read($tarHeap, read($tarHeap, getTarsBySrcs(Seq#Singleton(r)), RELSchema.relations), IndexField(j+_System.array.Length(read($srcHeap, r, ERSchema.entities))))): ref ==
+				getTarsBySrcs(Seq#Singleton( $Unbox(read($srcHeap, read($srcHeap, r, ERSchema.relships), IndexField(j))): ref) )
+			));
+// frame
+ensures (forall<alpha> $o: ref, $f: Field alpha :: 
+	$o != null && read(old($tarHeap), $o, alloc) ==>
+		( (dtype($o) == REL$RELSchema && dtype(Seq#Index(getTarsBySrcs_inverse($o), 0)) == ER$ERSchema && ($f == RELSchema.name || $f == RELSchema.relations)) || (read($tarHeap, $o, $f) == read(old($tarHeap), $o, $f))));
+ensures $HeapSucc(old($tarHeap), $tarHeap);
+ensures surj_tar_model($srcHeap, $tarHeap);
+		
+
+
+procedure E2R_applys();
+requires surj_tar_model($srcHeap, $tarHeap);
+requires (forall r: ref :: r!=null && read($srcHeap, r, alloc) && dtype(r) == ER$Entity ==>
+		read($tarHeap, getTarsBySrcs(Seq#Singleton(r)), alloc) 
+	 && getTarsBySrcs(Seq#Singleton(r)) != null 
+	 && dtype(getTarsBySrcs(Seq#Singleton(r))) == REL$Relation	);
+modifies $tarHeap;
+// t.name <- s.name
+ensures (forall r: ref :: r!=null && read($srcHeap, r, alloc) && dtype(r) == ER$Entity ==> 
+		read($tarHeap, getTarsBySrcs(Seq#Singleton(r)), Relation.name) == read($srcHeap, r, Entity.name));
+// dtype(t.attrs) = class._System.array
+ensures (forall r: ref :: r!=null && read($srcHeap, r, alloc) && dtype(r) == ER$Entity ==> 
+	dtype(read($tarHeap, getTarsBySrcs(Seq#Singleton(r)), Relation.attrs)) == class._System.array
+);
+// t.attrs != null && t.attrs.alloc
+ensures (forall r: ref :: r!=null && read($srcHeap, r, alloc) && dtype(r) == ER$Entity ==> 
+	read($tarHeap, getTarsBySrcs(Seq#Singleton(r)), Relation.attrs) != null 
+ && read($tarHeap, read($tarHeap, getTarsBySrcs(Seq#Singleton(r)), Relation.attrs), alloc)
+);
+// length(t.attrs) = length(s.attrs)
+ensures (forall r: ref :: r!=null && read($srcHeap, r, alloc) && dtype(r) == ER$Entity ==> 
+		_System.array.Length(read($tarHeap, getTarsBySrcs(Seq#Singleton(r)), Relation.attrs)) 
+	 == _System.array.Length(read($srcHeap, r, Entity.attrs))
+);
+// t.attrs[j] == s.attrs[j]
+ensures (forall r: ref :: r!=null && read($srcHeap, r, alloc) && dtype(r) == ER$Entity ==> 
+			( forall j: int :: 0<=j && j<_System.array.Length(read($srcHeap, r, Entity.attrs))  ==>
+				$Unbox(read($tarHeap, read($tarHeap, getTarsBySrcs(Seq#Singleton(r)), Relation.attrs), IndexField(j))): ref ==
+				getTarsBySrcs(Seq#Singleton( $Unbox(read($srcHeap, read($srcHeap, r, Entity.attrs), IndexField(j))): ref) )
+			));
+// frame property
+ensures (forall<alpha> $o: ref, $f: Field alpha :: 
+	$o != null && read(old($tarHeap), $o, alloc) ==>
+		((dtype($o) == REL$Relation && dtype(Seq#Index(getTarsBySrcs_inverse($o), 0)) == ER$Entity && ($f == Relation.name || $f == Relation.attrs)) || (read($tarHeap, $o, $f) == read(old($tarHeap), $o, $f))));
+ensures $HeapSucc(old($tarHeap), $tarHeap);
+ensures surj_tar_model($srcHeap, $tarHeap);
+
+procedure R2R_applys();
+requires surj_tar_model($srcHeap, $tarHeap);
+requires (forall r: ref :: r!=null && read($srcHeap, r, alloc) && dtype(r) == ER$Relship ==>
+		read($tarHeap, getTarsBySrcs(Seq#Singleton(r)), alloc) 
+	 && getTarsBySrcs(Seq#Singleton(r)) != null 
+	 && dtype(getTarsBySrcs(Seq#Singleton(r))) == REL$Relation	);
+modifies $tarHeap;
+// t.name <- s.name
+ensures (forall r: ref :: r!=null && read($srcHeap, r, alloc) && dtype(r) == ER$Relship ==> 
+		read($tarHeap, getTarsBySrcs(Seq#Singleton(r)), Relation.name) == read($srcHeap, r, Relship.name));
+// frame property
+ensures (forall<alpha> $o: ref, $f: Field alpha :: 
+	$o != null && read(old($tarHeap), $o, alloc) ==>
+		((dtype($o) == REL$Relation && dtype(Seq#Index(getTarsBySrcs_inverse($o), 0)) == ER$Relship && $f == Relation.name) || (read($tarHeap, $o, $f) == read(old($tarHeap), $o, $f))));
+ensures $HeapSucc(old($tarHeap), $tarHeap);
+ensures surj_tar_model($srcHeap, $tarHeap);
+
+
+procedure EA2A_applys();
+requires surj_tar_model($srcHeap, $tarHeap);
+requires (forall att,ent: ref :: 
+	att!=null && read($srcHeap, att, alloc) && dtype(att) == ER$ERAttribute 
+ && ent!=null && read($srcHeap, ent, alloc) && dtype(ent) == ER$Entity ==> 
+		read($srcHeap, att, ERAttribute.entity) == ent ==>
+		read($tarHeap, getTarsBySrcs(Seq#Build(Seq#Singleton(att),ent)), alloc) 
+	 && getTarsBySrcs(Seq#Build(Seq#Singleton(att),ent)) != null 
+	 && dtype(getTarsBySrcs(Seq#Build(Seq#Singleton(att),ent))) == REL$RELAttribute	); 
+modifies $tarHeap;
+ensures (forall att,ent: ref :: 
+	att!=null && read($srcHeap, att, alloc) && dtype(att) == ER$ERAttribute 
+ && ent!=null && read($srcHeap, ent, alloc) && dtype(ent) == ER$Entity ==> 
+		read($srcHeap, att, ERAttribute.entity) == ent ==>
+		read($tarHeap, getTarsBySrcs(Seq#Build(Seq#Singleton(att),ent)), RELAttribute.name) == read($srcHeap, att, ERAttribute.name));
+ensures (forall att,ent: ref :: 
+	att!=null && read($srcHeap, att, alloc) && dtype(att) == ER$ERAttribute 
+ && ent!=null && read($srcHeap, ent, alloc) && dtype(ent) == ER$Entity ==> 
+		read($srcHeap, att, ERAttribute.entity) == ent ==>
+		read($tarHeap, getTarsBySrcs(Seq#Build(Seq#Singleton(att),ent)), RELAttribute.isKey) == read($srcHeap, att, ERAttribute.isKey));
+ensures (forall<alpha> $o: ref, $f: Field alpha :: 
+	$o != null && read(old($tarHeap), $o, alloc) ==>
+		(  dtype($o) == REL$RELAttribute 
+		&& dtype(Seq#Index(getTarsBySrcs_inverse($o), 0)) == ER$ERAttribute 
+		&& dtype(Seq#Index(getTarsBySrcs_inverse($o), 1)) == ER$Entity 
+		&& ($f == RELAttribute.name || $f == RELAttribute.isKey)) 
+	 || (read($tarHeap, $o, $f) == read(old($tarHeap), $o, $f)));
+ensures $HeapSucc(old($tarHeap), $tarHeap);
+ensures surj_tar_model($srcHeap, $tarHeap);
+
+procedure RA2A_applys();
+requires surj_tar_model($srcHeap, $tarHeap);
+requires (forall att,rs: ref :: 
+	att!=null && read($srcHeap, att, alloc) && dtype(att) == ER$ERAttribute 
+ && rs!=null && read($srcHeap, rs, alloc) && dtype(rs) == ER$Relship ==> 
+		read($srcHeap, att, ERAttribute.relship) == rs ==>
+		read($tarHeap, getTarsBySrcs(Seq#Build(Seq#Singleton(att),rs)), alloc) 
+	 && getTarsBySrcs(Seq#Build(Seq#Singleton(att),rs)) != null 
+	 && dtype(getTarsBySrcs(Seq#Build(Seq#Singleton(att),rs))) == REL$RELAttribute	);	
+modifies $tarHeap;
+ensures (forall att,rs: ref :: 
+	att!=null && read($srcHeap, att, alloc) && dtype(att) == ER$ERAttribute 
+ && rs!=null && read($srcHeap, rs, alloc) && dtype(rs) == ER$Relship ==> 
+		read($srcHeap, att, ERAttribute.relship) == rs ==>
+		read($tarHeap, getTarsBySrcs(Seq#Build(Seq#Singleton(att),rs)), RELAttribute.name) == read($srcHeap, att, ERAttribute.name));
+ensures (forall att,rs: ref :: 
+	att!=null && read($srcHeap, att, alloc) && dtype(att) == ER$ERAttribute 
+ && rs!=null && read($srcHeap, rs, alloc) && dtype(rs) == ER$Relship ==> 
+		read($srcHeap, att, ERAttribute.relship) == rs ==>
+		read($tarHeap, getTarsBySrcs(Seq#Build(Seq#Singleton(att),rs)), RELAttribute.isKey) == read($srcHeap, att, ERAttribute.isKey));
+ensures (forall att,rs: ref :: 
+	att!=null && read($srcHeap, att, alloc) && dtype(att) == ER$ERAttribute 
+ && rs!=null && read($srcHeap, rs, alloc) && dtype(rs) == ER$Relship ==> 
+		read($srcHeap, att, ERAttribute.relship) == rs ==>
+		read($tarHeap, getTarsBySrcs(Seq#Build(Seq#Singleton(att),rs)), RELAttribute.relation) == getTarsBySrcs(Seq#Singleton(rs)));
+ensures (forall<alpha> $o: ref, $f: Field alpha :: 
+	$o != null && read(old($tarHeap), $o, alloc) ==>
+		(  dtype($o) == REL$RELAttribute 
+		&& dtype(Seq#Index(getTarsBySrcs_inverse($o), 0)) == ER$ERAttribute 
+		&& dtype(Seq#Index(getTarsBySrcs_inverse($o), 1)) == ER$Relship 
+		&& ($f == RELAttribute.name || $f == RELAttribute.isKey || $f == RELAttribute.relation)) 
+	 || (read($tarHeap, $o, $f) == read(old($tarHeap), $o, $f)));
+ensures $HeapSucc(old($tarHeap), $tarHeap);
+ensures surj_tar_model($srcHeap, $tarHeap);
+
+procedure RA2AK_applys();
+requires surj_tar_model($srcHeap, $tarHeap);
+requires (forall att,rs: ref :: 
+	att!=null && read($srcHeap, att, alloc) && dtype(att) == ER$ERAttribute 
+ && rs!=null && read($srcHeap, rs, alloc) && dtype(rs) == ER$Relship ==> 
+		read($srcHeap, att, ERAttribute.relship) == rs ==>
+		read($tarHeap, getTarsBySrcs(Seq#Build(Seq#Singleton(att),rs)), alloc) 
+	 && getTarsBySrcs(Seq#Build(Seq#Singleton(att),rs)) != null 
+	 && dtype(getTarsBySrcs(Seq#Build(Seq#Singleton(att),rs))) == REL$RELAttribute	);	
+modifies $tarHeap;
+ensures (forall att,rs: ref :: 
+	att!=null && read($srcHeap, att, alloc) && dtype(att) == ER$ERAttribute 
+ && rs!=null && read($srcHeap, rs, alloc) && dtype(rs) == ER$Relship ==> 
+		read($srcHeap, att, ERAttribute.relship) == rs ==>
+		read($tarHeap, getTarsBySrcs(Seq#Build(Seq#Singleton(att),rs)), RELAttribute.name) == read($srcHeap, att, ERAttribute.name));
+ensures (forall att,rs: ref :: 
+	att!=null && read($srcHeap, att, alloc) && dtype(att) == ER$ERAttribute 
+ && rs!=null && read($srcHeap, rs, alloc) && dtype(rs) == ER$Relship ==> 
+		read($srcHeap, att, ERAttribute.relship) == rs ==>
+		read($tarHeap, getTarsBySrcs(Seq#Build(Seq#Singleton(att),rs)), RELAttribute.isKey) == read($srcHeap, att, ERAttribute.isKey));
+ensures (forall att,rs: ref :: 
+	att!=null && read($srcHeap, att, alloc) && dtype(att) == ER$ERAttribute 
+ && rs!=null && read($srcHeap, rs, alloc) && dtype(rs) == ER$Relship ==> 
+		read($srcHeap, att, ERAttribute.relship) == rs ==>
+		read($tarHeap, getTarsBySrcs(Seq#Build(Seq#Singleton(att),rs)), RELAttribute.relation) == getTarsBySrcs(Seq#Singleton(rs)));
+ensures (forall<alpha> $o: ref, $f: Field alpha :: 
+	$o != null && read(old($tarHeap), $o, alloc) ==>
+		(  dtype($o) == REL$RELAttribute 
+		&& dtype(Seq#Index(getTarsBySrcs_inverse($o), 0)) == ER$ERAttribute 
+		&& dtype(Seq#Index(getTarsBySrcs_inverse($o), 1)) == ER$Relship 
+		&& ($f == RELAttribute.name || $f == RELAttribute.isKey || $f == RELAttribute.relation)) 
+	 || (read($tarHeap, $o, $f) == read(old($tarHeap), $o, $f)));
+ensures $HeapSucc(old($tarHeap), $tarHeap);
+ensures surj_tar_model($srcHeap, $tarHeap);
